cedar-lean/Cedar/Thm/Validation/Slice/Reachable/BinaryApp.lean
@@ -55,7 +55,7 @@ theorem reachable_tag_step {n : Nat} {euid euid' : EntityUID} {start : Set Entit
 
 theorem checked_eval_entity_reachable_get_tag {e₁ e₂: Expr} {n : Nat} {c c' : Capabilities} {tx : TypedExpr} {env : Environment} {entities : Entities} {path : List Attr}
   (hc : CapabilitiesInvariant c request entities)
-  (hr : RequestAndEntitiesMatchEnvironment env request entities)
+  (hr : InstanceOfWellFormedEnvironment request entities env)
   (ht : typeOf (.binaryApp .getTag e₁ e₂) c env = .ok (tx, c'))
   (hl : tx.EntityAccessAtLevel env n nmax path)
   (he : evaluate (.binaryApp .getTag e₁ e₂) request entities = .ok v)
@@ -111,7 +111,7 @@ theorem binary_op_not_euid_via_path {op : BinaryOp} {e₁ e₂: Expr} {entities 
 
 theorem checked_eval_entity_reachable_binary {op : BinaryOp} {e₁ e₂: Expr} {n : Nat} {c c' : Capabilities} {tx : TypedExpr} {env : Environment} {entities : Entities} {path : List Attr}
   (hc : CapabilitiesInvariant c request entities)
-  (hr : RequestAndEntitiesMatchEnvironment env request entities)
+  (hr : InstanceOfWellFormedEnvironment request entities env)
   (ht : typeOf (.binaryApp op e₁ e₂) c env = .ok (tx, c'))
   (hl : tx.EntityAccessAtLevel env n nmax path)
   (he : evaluate (.binaryApp op e₁ e₂) request entities = .ok v)
