cedar-lean/Cedar/Thm/Validation/Typechecker/WF.lean
@@ -1,0 +1,293 @@
+/-
+ Copyright Cedar Contributors
+
+ Licensed under the Apache License, Version 2.0 (the "License");
+ you may not use this file except in compliance with the License.
+ You may obtain a copy of the License at
+
+      https://www.apache.org/licenses/LICENSE-2.0
+
+ Unless required by applicable law or agreed to in writing, software
+ distributed under the License is distributed on an "AS IS" BASIS,
+ WITHOUT WARRANTIES OR CONDITIONS OF ANY KIND, either express or implied.
+ See the License for the specific language governing permissions and
+ limitations under the License.
+-/
+
+import Cedar.Spec
+import Cedar.Validation
+
+/-!
+This file contains the definition of well-formedness of `Environment`
+and related definitions.
+--/
+
+namespace Cedar.Validation
+
+open Cedar.Data
+open Cedar.Validation
+open Cedar.Spec
+
+----- Well-formedness of environment -----
+
+def ActionSchema.IsActionEntityType (acts : ActionSchema) (ety : EntityType) : Prop :=
+  ∃ uid, acts.contains uid ∧ uid.ty = ety
+
+/--
+Either a non-action entity type in `env.ets`,
+or an action entity type in `env.acts`.
+-/
+def EntityType.WellFormed (env : Environment) (ety : EntityType) : Prop :=
+  env.ets.contains ety ∨ env.acts.IsActionEntityType ety
+
+mutual
+inductive QualifiedType.WellFormed (env : Environment) : Qualified CedarType → Prop where
+  | optional_wf {ty : CedarType}
+    (h : CedarType.WellFormed env ty) :
+    QualifiedType.WellFormed env (.optional ty)
+  | required_wf {ty : CedarType}
+    (h : CedarType.WellFormed env ty) :
+    QualifiedType.WellFormed env (.required ty)
+
+/--
+Defines when a `CedarType` is well-formed in an `Environment`.
+-/
+inductive CedarType.WellFormed (env : Environment) : CedarType → Prop where
+  | bool_wf {bty : BoolType} : CedarType.WellFormed env (.bool bty)
+  | int_wf : CedarType.WellFormed env .int
+  | string_wf : CedarType.WellFormed env .string
+  | entity_wf {ety : EntityType}
+    (h : EntityType.WellFormed env ety) :
+    CedarType.WellFormed env (.entity ety)
+  | set_wf {ty : CedarType}
+    (h : CedarType.WellFormed env ty) :
+    CedarType.WellFormed env (.set ty)
+  | record_wf {rty : RecordType}
+    -- Well-formed as a `Map`
+    (h₁ : rty.WellFormed)
+    -- Each attribute type is well-formed
+    (h₂ : ∀ attr qty, rty.find? attr = some qty → QualifiedType.WellFormed env qty) :
+    CedarType.WellFormed env (.record rty)
+  | ext_wf {xty : ExtType} : CedarType.WellFormed env (.ext xty)
+end
+
+def StandardSchemaEntry.WellFormed (env : Environment) (entry : StandardSchemaEntry) : Prop :=
+  -- Well-formed as `Map`/`Set`s
+  entry.ancestors.WellFormed ∧
+  -- Each ancestor entity type must be a well-formed,
+  -- non-action, non-enum entity type
+  (∀ anc ∈ entry.ancestors,
+    ∃ entry, env.ets.find? anc = some entry ∧ entry.isStandard) ∧
+  -- The attribute types are well-formed
+  (CedarType.record entry.attrs).WellFormed env ∧
+  -- The tag type is well-formed
+  (∀ ty, entry.tags = .some ty → CedarType.WellFormed env ty)
+
+def EntitySchemaEntry.WellFormed (env : Environment) (entry : EntitySchemaEntry) : Prop :=
+  match entry with
+  | standard entry => entry.WellFormed env
+  | enum es => es.WellFormed ∧ ¬es.isEmpty
+
+def EntitySchema.WellFormed (env : Environment) (ets : EntitySchema) : Prop :=
+  Map.WellFormed ets ∧
+  ∀ ety entry, ets.find? ety = some entry → entry.WellFormed env
+
+def EntityUID.WellFormed (env : Environment) (uid : EntityUID) : Prop :=
+  env.ets.isValidEntityUID uid ∨ env.acts.contains uid
+
+def ActionSchemaEntry.WellFormed (env : Environment) (entry : ActionSchemaEntry) : Prop :=
+  -- Well-formed as `Map`/`Set`s
+  entry.appliesToPrincipal.WellFormed ∧
+  entry.appliesToResource.WellFormed ∧
+  entry.ancestors.WellFormed ∧
+  -- Each principal/resource entity type is well-formed
+  (∀ ety, entry.appliesToPrincipal.contains ety → EntityType.WellFormed env ety) ∧
+  (∀ ety, entry.appliesToResource.contains ety → EntityType.WellFormed env ety) ∧
+  -- Ancestors of each action entity must also be an action entity
+  (∀ uid ∈ entry.ancestors, env.acts.contains uid) ∧
+  -- Context is a well-formed `RecordType`
+  (CedarType.record entry.context).WellFormed env
+
+def ActionSchema.AcyclicActionHierarchy (acts : ActionSchema) : Prop :=
+  ∀ uid entry, acts.find? uid = .some entry → uid ∉ entry.ancestors
+
+def ActionSchema.TransitiveActionHierarchy (acts : ActionSchema) : Prop :=
+  ∀ uid₁ entry₁ uid₂ entry₂,
+    acts.find? uid₁ = .some entry₁ →
+    acts.find? uid₂ = .some entry₂ →
+    uid₂ ∈ entry₁.ancestors →
+    entry₂.ancestors ⊆ entry₁.ancestors
+
+def ActionSchema.WellFormed (env : Environment) (acts : ActionSchema) : Prop :=
+  Map.WellFormed acts ∧
+  (∀ uid entry, acts.find? uid = some entry → entry.WellFormed env) ∧
+  (∀ uid, acts.contains uid → ¬env.ets.contains uid.ty) ∧
+  acts.AcyclicActionHierarchy ∧
+  acts.TransitiveActionHierarchy
+
+def RequestType.WellFormed (env : Environment) (reqty : RequestType) : Prop :=
+  ∃ entry, env.acts.find? reqty.action = some entry ∧
+    -- Enforce that principal/resource/context are valid for the action
+    reqty.principal ∈ entry.appliesToPrincipal ∧
+    reqty.resource ∈ entry.appliesToResource ∧
+    reqty.context = entry.context
+  -- Other properties, such as the well-formedness of principal/resource/context
+  -- follows from the above and the well-formedness of `env.ets` and `env.acts`.
+
+def Environment.WellFormed (env : Environment) : Prop :=
+  env.ets.WellFormed env ∧
+  env.acts.WellFormed env ∧
+  env.reqty.WellFormed env
+
+----- Some lemmas -----
+
+theorem qty_wf_implies_type_of_wf {env : Environment} {qty : Qualified CedarType}
+  (h : QualifiedType.WellFormed env qty) :
+  CedarType.WellFormed env qty.getType
+:= by
+  cases h with
+  | optional_wf hwf => simp [Qualified.getType, hwf]
+  | required_wf hwf => simp [Qualified.getType, hwf]
+
+theorem wf_record_type_cons {env : Environment}
+  {hd : (Attr × Qualified CedarType)}
+  {tl : List (Attr × Qualified CedarType)}
+  (hwf : CedarType.WellFormed env (.record (Map.mk (hd :: tl)))) :
+  CedarType.WellFormed env hd.snd.getType ∧
+  CedarType.WellFormed env (.record (Map.mk tl))
+:= by
+  cases hwf
+  rename_i hwf_map hwf_tys
+  simp only [Map.WellFormed] at hwf_map
+  constructor
+  · have := hwf_tys hd.fst hd.snd
+    simp only [Map.find?, List.find?, BEq.rfl, forall_const] at this
+    cases e : hd.snd
+    all_goals
+      simp only [e] at *
+      cases this
+      simp only [Qualified.getType]
+      assumption
+  · constructor
+    · simp only [Map.WellFormed]
+      apply Eq.symm
+      apply Map.make_eq_mk.mp
+      have := Map.make_eq_mk.mpr (Eq.symm hwf_map)
+      cases this with
+      | cons_nil => constructor
+      | cons_cons =>
+        simp only [Map.toList, Map.kvs]
+        assumption
+    · intros attr qty hfound
+      have hfound := Map.find?_mem_toList hfound
+      simp only [Map.toList, Map.kvs] at hfound
+      have : (Map.mk (hd :: tl)).find? attr = some qty := by
+        apply (Map.in_list_iff_find?_some ?_).mp
+        · simp [Map.kvs, hfound]
+        · simp only [Map.WellFormed]
+          assumption
+      exact hwf_tys attr qty this
+
+theorem wf_record_implies_wf_attr {env : Environment} {rty : RecordType} {attr : Attr} {qty : QualifiedType}
+  (hwf : CedarType.WellFormed env (.record rty))
+  (hqty : rty.find? attr = some qty) :
+  QualifiedType.WellFormed env qty
+:= by
+  cases hwf with
+  | record_wf _ hattr =>
+    exact hattr attr qty hqty
+
+theorem wf_env_implies_wf_entity_schema_entry {env : Environment} {ety : EntityType} {entry : EntitySchemaEntry}
+  (hwf : env.WellFormed)
+  (hets : env.ets.find? ety = some entry) :
+  entry.WellFormed env
+:= by
+  have ⟨⟨_, hwf_ets⟩, _⟩ := hwf
+  exact hwf_ets ety entry hets
+
+theorem wf_env_implies_wf_tag_type {env : Environment} {ety : EntityType} {ty : CedarType}
+  (hwf : env.WellFormed)
+  (hety : env.ets.tags? ety = .some (.some ty)) :
+  CedarType.WellFormed env ty
+:= by
+  simp only [EntitySchema.tags?, Option.map_eq_some_iff] at hety
+  have ⟨entry, hentry, htags⟩ := hety
+  have ⟨⟨_, hwf_ets⟩, _⟩ := hwf
+  have hwf_entry := hwf_ets ety entry hentry
+  simp only [EntitySchemaEntry.WellFormed] at hwf_entry
+  split at hwf_entry
+  · have ⟨_, _, _, hwf_tag⟩ := hwf_entry
+    simp only [EntitySchemaEntry.tags?] at htags
+    exact hwf_tag ty htags
+  · simp [EntitySchemaEntry.tags?] at htags
+
+theorem wf_env_implies_wf_attrs {env : Environment} {ety : EntityType} {attrs : RecordType}
+  (hwf : env.WellFormed)
+  (hattrs : env.ets.attrs? ety = .some attrs) :
+  CedarType.WellFormed env (.record attrs)
+:= by
+  simp only [EntitySchema.attrs?, Option.map_eq_some_iff] at hattrs
+  have ⟨entry, hentry, hattrs⟩ := hattrs
+  have ⟨⟨_, hwf_ets⟩, _⟩ := hwf
+  have hwf_entry := hwf_ets ety entry hentry
+  simp only [EntitySchemaEntry.WellFormed] at hwf_entry
+  split at hwf_entry
+  · have ⟨_, _, hwf_attrs, _⟩ := hwf_entry
+    simp only [← hattrs]
+    exact hwf_attrs
+  · simp only [EntitySchemaEntry.attrs] at hattrs
+    simp only [← hattrs, Map.empty]
+    constructor
+    . simp [Map.WellFormed, Map.toList, Map.kvs, Map.make, List.canonicalize]
+    · simp [Map.find?, List.find?]
+
+theorem wf_env_implies_action_wf {env : Environment}
+  (hwf : env.WellFormed) :
+  EntityUID.WellFormed env env.reqty.action
+:= by
+  have ⟨_, _, hwf_req⟩ := hwf
+  have ⟨_, hact, _⟩ := hwf_req
+  apply Or.inr
+  simp [EntityUID.WellFormed, ActionSchema.contains, hact]
+
+theorem wf_env_disjoint_ets_acts
+  {env : Environment} {uid : EntityUID}
+  {ets_entry : EntitySchemaEntry}
+  {acts_entry : ActionSchemaEntry}
+  (hwf : env.WellFormed)
+  (hets : env.ets.find? uid.ty = some ets_entry)
+  (hacts : env.acts.find? uid = some acts_entry) :
+  False
+:= by
+  have ⟨_, ⟨_, _, hdisj, _⟩, _⟩ := hwf
+  have := hdisj uid
+  apply this
+  · simp [ActionSchema.contains, hacts]
+  · simp [EntitySchema.contains, hets]
+
+/--
+More well-formedness properties of `env.reqty`.
+-/
+theorem wf_env_implies_wf_request
+  {env : Environment}
+  (hwf : env.WellFormed) :
+  EntityType.WellFormed env env.reqty.principal ∧
+  env.acts.contains env.reqty.action ∧
+  EntityType.WellFormed env env.reqty.resource ∧
+  (CedarType.record env.reqty.context).WellFormed env
+:= by
+  have ⟨_, hwf_acts, ⟨entry, hwf_act, hwf_princ, hwf_res, hwf_ctx⟩⟩ := hwf
+  have ⟨_, hwf_acts, _⟩ := hwf_acts
+  have hwf_act_entry := hwf_acts env.reqty.action entry hwf_act
+  have ⟨_, _, _, hwf_app_to_princ, hwf_app_to_res, _, hwf_ctx_ty⟩ := hwf_act_entry
+  and_intros
+  · apply hwf_app_to_princ
+    simp only [Membership.mem] at hwf_princ
+    simp [Set.contains, hwf_princ, Membership.mem]
+  · simp [ActionSchema.contains, hwf_act]
+  · apply hwf_app_to_res
+    simp only [Membership.mem] at hwf_res
+    simp [Set.contains, hwf_res, Membership.mem]
+  · simp [hwf_ctx, hwf_ctx_ty]
+
+end Cedar.Validation
