cedar-lean/Cedar/Thm/Validation/WellTyped/WF.lean
@@ -1,0 +1,188 @@
+/-
+ Copyright Cedar Contributors
+
+ Licensed under the Apache License, Version 2.0 (the "License");
+ you may not use this file except in compliance with the License.
+ You may obtain a copy of the License at
+
+      https://www.apache.org/licenses/LICENSE-2.0
+
+ Unless required by applicable law or agreed to in writing, software
+ distributed under the License is distributed on an "AS IS" BASIS,
+ WITHOUT WARRANTIES OR CONDITIONS OF ANY KIND, either express or implied.
+ See the License for the specific language governing permissions and
+ limitations under the License.
+-/
+
+import Cedar.Thm.Validation.WellTyped.Definition
+import Cedar.Thm.Validation.WellTyped.Typechecking
+import Cedar.Thm.Validation.WellTyped.TypeLifting
+import Cedar.Thm.Validation.Typechecker.WF
+
+/-!
+This file contains the theorems that `TypedExpr.WellTyped` implies `CedarType.WellFormed`.
+-/
+
+namespace Cedar.Thm
+
+open Cedar.Data
+open Cedar.Validation
+open Cedar.Spec
+
+/--
+`TypedExpr.WellTyped` implies well-formedness of the type (`CedarType.WellFormed`).
+-/
+theorem well_typed_implies_wf_type
+  {env : Environment} {tx : TypedExpr}
+  (hwf_env : env.WellFormed)
+  (hwt : TypedExpr.WellTyped env tx) :
+  CedarType.WellFormed env tx.typeOf
+:= by
+  cases hwt with
+  | lit hwt_prim =>
+    cases hwt_prim
+    any_goals
+      simp only [TypedExpr.typeOf]
+      constructor
+    rename_i hwt_uid
+    simp only [EntityType.WellFormed, ActionSchema.IsActionEntityType]
+    simp only [EntitySchema.isValidEntityUID] at hwt_uid
+    rcases hwt_uid with hets | hacts
+    · split at hets
+      · rename_i hsome
+        simp [EntitySchema.contains, Map.contains, Option.isSome, hsome]
+      · contradiction
+    · rename_i uid
+      apply Or.inr
+      exists uid
+  | var hwt_var =>
+    have ⟨hwf_principal, hwf_action, hwf_resource, hwf_context⟩
+    := wf_env_implies_wf_request hwf_env
+    cases hwt_var
+    all_goals simp only [TypedExpr.typeOf]
+    case principal =>
+      constructor
+      assumption
+    case action =>
+      constructor
+      simp only [EntityType.WellFormed, ActionSchema.IsActionEntityType]
+      apply Or.inr
+      exists env.reqty.action
+    case resource =>
+      constructor
+      assumption
+    case context =>
+      apply wf_type_iff_wf_liftBoolTypes.mp
+      assumption
+  | ite _ hwf2 =>
+    simp only [TypedExpr.typeOf]
+    exact well_typed_implies_wf_type hwf_env hwf2
+  | and _ => constructor
+  | or _ => constructor
+  | unaryApp _ hwt_op =>
+    simp only [TypedExpr.typeOf]
+    cases hwt_op
+    all_goals constructor
+  | binaryApp _ _ hwt_op =>
+    simp only [TypedExpr.typeOf]
+    cases hwt_op with
+    | getTag =>
+      apply wf_type_iff_wf_liftBoolTypes.mp
+      apply wf_env_implies_wf_tag_type
+      assumption
+      assumption
+    | _ => constructor
+  | hasAttr_entity => constructor
+  | hasAttr_record => constructor
+  | getAttr_entity _ _ hattrs hattr =>
+    simp only [TypedExpr.typeOf]
+    simp only [Option.map_eq_some_iff] at hattrs hattr
+    have ⟨attrs, hattrs, hattrs_lift⟩ := hattrs
+    have ⟨attr, hattr, hattr_ty⟩ := hattr
+    simp only [← hattr_ty]
+    have hwf_attrs := wf_env_implies_wf_attrs hwf_env hattrs
+    have hwf_attrs_lift := wf_type_iff_wf_liftBoolTypes.mp hwf_attrs
+    simp only [CedarType.liftBoolTypes, hattrs_lift] at hwf_attrs_lift
+    have hwf_attr := wf_record_implies_wf_attr hwf_attrs_lift hattr
+    apply qty_wf_implies_type_of_wf
+    exact hwf_attr
+  | getAttr_record hwt1 hwt_rec hattr =>
+    simp only [TypedExpr.typeOf]
+    simp only [Option.map_eq_some_iff] at hattr
+    have hwf1 := well_typed_implies_wf_type hwf_env hwt1
+    simp only [hwt_rec] at hwf1
+    have ⟨attr, hattr, hattr_ty⟩ := hattr
+    simp only [← hattr_ty]
+    apply qty_wf_implies_type_of_wf
+    apply wf_record_implies_wf_attr
+    assumption
+    assumption
+  | set hwt_elem hty_elem hnon_empty =>
+    rename_i elems elem_ty
+    simp only [TypedExpr.typeOf]
+    constructor
+    cases elems with
+    | nil => contradiction
+    | cons hd _ =>
+      have := hwt_elem hd
+      simp only [List.mem_cons, true_or, forall_const] at this
+      have hwf_hd := well_typed_implies_wf_type hwf_env this
+      have := hty_elem hd
+      simp only [List.mem_cons, true_or, forall_const] at this
+      simp only [this] at hwf_hd
+      assumption
+  | record hwt_attrs hrty =>
+    simp only [TypedExpr.typeOf]
+    rename_i rty attrs_ls
+    have hwf_rty : Map.WellFormed rty := by
+      simp only [hrty]
+      apply Map.make_wf
+    constructor
+    · exact hwf_rty
+    · intros attr qty hattr
+      have := (Map.in_list_iff_find?_some hwf_rty).mpr hattr
+      simp only [hrty] at this
+      have := Map.make_mem_list_mem this
+      simp only [List.mem_map, Prod.mk.injEq, Prod.exists] at this
+      have ⟨attr, tx, htx, heq_attr, hqty⟩ := this
+      have := hwt_attrs attr tx htx
+      -- For termination
+      have _ : sizeOf tx < 1 + sizeOf attrs_ls + (1 + sizeOf rty) := by
+        simp [*]
+        have h := List.sizeOf_snd_lt_sizeOf_list htx
+        simp at h
+        omega
+      have := well_typed_implies_wf_type hwf_env this
+      simp only [← hqty]
+      constructor
+      assumption
+  | call _ hwt_xfn =>
+    cases hwt_xfn
+    all_goals
+      simp only [TypedExpr.typeOf]
+      constructor
+
+/--
+The result of `typeOf` has a well-formed type.
+-/
+theorem typechecked_has_well_formed_type
+  {e : Expr}
+  {c₁ c₂ : Capabilities}
+  {env : Environment}
+  {tx : TypedExpr}
+  (hwf : env.WellFormed)
+  (hty : typeOf e c₁ env = .ok (tx, c₂)) :
+  tx.typeOf.WellFormed env
+:= by
+  have : CedarType.WellFormed env tx.liftBoolTypes.typeOf := by
+    apply well_typed_implies_wf_type hwf
+    apply typechecked_is_well_typed_after_lifting
+    assumption
+  cases tx
+  all_goals
+    simp only [TypedExpr.liftBoolTypes, TypedExpr.typeOf] at this
+    simp only [TypedExpr.typeOf]
+    apply wf_type_iff_wf_liftBoolTypes.mpr
+    assumption
+
+end Cedar.Thm
